Wrote all the missing versions of quicksort and mergesort and refactored their files to make names match. Proved a small lemma about sortedness.

Quicksort.v
@@ -23,32 +23,125 @@ Qed.
 Hint Resolve le_n_S filter_length.
 
 (* Quicksort using Program Fixpoint *)
-Program Fixpoint qs (A : LinDec) (l : list A) {measure (length l)} : list A :=
+Program Fixpoint qsPF (A : LinDec) (l : list A) {measure (length l)}
+    : list A :=
 match l with
-    | nil => nil
-    | h :: t => qs A (filter (fun x : A => leqb x h) t) ++ [h]
-             ++ qs A (filter (fun x : A => negb (leqb x h)) t)
+    | [] => []
+    | h :: t => qsPF A (filter (fun x : A => leqb x h) t) ++ [h]
+             ++ qsPF A (filter (fun x : A => negb (leqb x h)) t)
 end.
 Next Obligation. simpl. unfold lt. auto. Qed.
 Next Obligation. simpl. unfold lt. auto. Qed.
 
-Eval compute in (qs natle testl).
+Eval compute in qsPF natle testl.
+
+(* Quicksort using Function. *)
+Function qsFun (A : LinDec) (l : list A) {measure length l} : list A :=
+match l with
+    | [] => []
+    | h :: t => qsFun A (filter (fun x : A => leqb x h) t) ++
+           h :: qsFun A (filter (fun x : A => negb (leqb x h)) t)
+end.
+Proof.
+  intros. unfold lt. simpl. apply le_n_S. apply filter_length.
+  intros. unfold lt. simpl. apply le_n_S. apply filter_length.
+Defined.
+
+Eval compute in qsFun natle testl.
+
+Lemma sorted_inv2 :
+  forall (A : LinDec) (x y : A) (l : list A),
+    sorted A (x :: y :: l) -> leq x y.
+Proof.
+  inversion 1; subst. assumption.
+Qed.
+
+Lemma sorted_app_all :
+  forall (A : LinDec) (l : list A) (h : A) (t : list A),
+    sorted A l -> sorted A (h :: t) -> (forall x : A, In x l -> leq x h) ->
+      sorted A (l ++ h :: t).
+Proof.
+  induction l as [| h t]; simpl; intros.
+    assumption.
+    destruct t as [| h' t'].
+      simpl in *. constructor.
+        eapply (H1 h); eauto.
+        assumption.
+      rewrite <- app_comm_cons. constructor.
+        eapply sorted_inv2. eassumption.
+        apply IHt.
+          apply sorted_inv with h. assumption.
+          assumption.
+          intros. apply H1. right. assumption.
+Qed.
+
+Theorem qsFun_sorted :
+  forall (A : LinDec) (l : list A), sorted A (qsFun A l).
+Proof.
+  intros. functional induction (@qsFun A) l.
+    constructor.
+    apply sorted_app_all.
+      assumption.
+      Focus 2. intros.
+Abort. (* TODO : *)
 
 (* Quicksort using fuel recursion. *)
-Fixpoint qsortSub (A : LinDec) (fuel : nat) (l : list A) : list A :=
+Fixpoint qsFuel' (A : LinDec) (fuel : nat) (l : list A) : list A :=
 match fuel, l with
     | 0, _ => l
     | _, [] => []
     | _, [x] => [x]
     | S fuel', h :: t =>
-        let lesser := qsortSub A fuel' (filter (fun x : A => leqb x h) t) in
-        let greater := qsortSub A fuel' (filter (fun x : A => negb (leqb x h)) t) in
-        lesser ++ [h] ++ greater
+        qsFuel' A fuel' (filter (fun x : A => leqb x h) t) ++ h ::
+        qsFuel' A fuel' (filter (fun x : A => negb (leqb x h)) t)
 end.
 
-Definition qs' (A : LinDec) (l : list A) : list A := qsortSub A (length l) l.
+Definition qsFuel (A : LinDec) (l : list A) : list A :=
+    qsFuel' A (length l) l.
 
-Eval compute in (qs' natle testl).
+Eval compute in (qsFuel natle testl).
+
+(* Quicksort using well-founded recursion. *)
+
+Lemma filter_lengthOrder :
+  forall {A : Type} (p : A -> bool) (h : A) (t : list A),
+    lengthOrder (filter p t) (h :: t).
+Proof.
+  intros. unfold lengthOrder, lt. simpl. apply le_n_S.
+  apply filter_length.
+Qed.
+
+Definition qsWf (A : LinDec) : list A -> list A.
+Proof.
+  apply (Fix (@lengthOrder_wf A) _).
+  intros l qsWf.
+  destruct l as [| h t].
+    exact [].
+    pose (le := qsWf (filter (fun x : A => leqb x h) t)
+        (filter_lengthOrder (fun x => leqb x h) h t)).
+    pose (gt := qsWf (filter (fun x : A => negb (leqb x h)) t)
+        (filter_lengthOrder (fun x : A => negb (leqb x h)) h t)).
+    exact (le ++ h :: gt).
+Defined.
+
+Eval compute in qsWf natle testl.
+
+(* Quicksort using wel-founded recursion and refine. *)
+
+Definition qsWfRef (A : LinDec) : list A -> list A.
+refine (Fix (@lengthOrder_wf A) _ (fun (l : list A) =>
+match l with
+    | [] => fun _ => []
+    | h :: t => fun qs =>
+        qs (filter (fun x : A => leqb x h) t) _ ++ h ::
+        qs (filter (fun x : A => negb (leqb x h)) t) _
+end)).
+Proof.
+  apply filter_lengthOrder.
+  apply filter_lengthOrder.
+Defined.
+
+Eval compute in qsWfRef natle testl.
 
 (* Quicksort using Bove-Capretta *)
 
@@ -61,37 +154,54 @@ Inductive qsDom {A : LinDec} : list A -> Type :=
         qsDom (filter (fun x : A => negb (leqb x h)) t) ->
         qsDom (h :: t).
 
-Fixpoint qs3' (A : LinDec) (l : list A) (dom : qsDom l) : list A :=
+Fixpoint qsBC' (A : LinDec) (l : list A) (dom : qsDom l) : list A :=
 match dom with
     | qsDom0 => nil
     | qsDom1 h t dom1 dom2 =>
-        qs3' A (filter (fun x : A => leqb x h) t) dom1 ++ h ::
-        qs3' A (filter (fun x : A => negb (leqb x h)) t) dom2
+        qsBC' A (filter (fun x : A => leqb x h) t) dom1 ++ h ::
+        qsBC' A (filter (fun x : A => negb (leqb x h)) t) dom2
 end.
 
 Theorem all_qsDom : forall (A : LinDec) (l : list A), qsDom l.
 Proof.
   intro. apply well_founded_induction_type with lengthOrder.
     apply lengthOrder_wf.
-    intros. destruct x as [| h t]; constructor.
-      apply X. simpl. unfold lt. apply le_n_S. apply filter_length.
-      apply X. simpl. unfold lt. apply le_n_S. apply filter_length.
+    intros. destruct x as [| h t]; constructor; apply X.
+      simpl. unfold lt. apply le_n_S. apply filter_length.
+      simpl. unfold lt. apply le_n_S. apply filter_length.
 Defined.
 
-Definition qs3 (A : LinDec) (l : list A) : list A :=
-    qs3' A l (all_qsDom A l).
+Definition qsBC (A : LinDec) (l : list A) : list A :=
+    qsBC' A l (all_qsDom A l).
 
-Eval compute in qs3 natle testl.
+Eval compute in qsBC natle testl.
+
+(* nb_occ lemmas *)
+
+Lemma nb_occ_reverse :
+  forall (A : LinDec) (l : list A) (x : A),
+    nb_occ A x (rev l) = nb_occ A x l.
+Proof.
+  induction l as [| h t].
+    simpl; intros; reflexivity.
+    intros. SearchAbout rev_append. rewrite rev_alt. simpl.
+Abort.
 
 (* Tried to prove that quicksort gives a permutation, but failed. *)
-(*Lemma nb_occ_app : forall (A : LinDec) (l1 l2 : list A) (x : A),
-    nb_occ A x (l1 ++ l2) = nb_occ A x (l2 ++ l1).
+Lemma nb_occ_app : forall (A : LinDec) (x : A) (l1 l2 l3 : list A),
+    l3 = l1 ++ l2 -> nb_occ A x (l1 ++ l2) = nb_occ A x (l2 ++ l1).
 Proof.
-  induction l1 as [| h t]; induction l2 as [| h' t']; simpl;
-  intros; repeat rewrite app_nil_r; auto. simpl in *.
-  case_eq (LinDec_eq x h); case_eq (LinDec_eq x h'); intros.
-  f_equal. assert (h = h'). unfold LinDec_eq in H. 
-    
+  induction l1 as [| h1 t1].
+    simpl; intros. rewrite app_nil_r. reflexivity.
+    intros. rewrite <- app_comm_cons at 1.
+      replace (l2 ++ h1 :: t1) with ((l2 ++ [h1]) ++ t1). (*
+        rewrite <- IHt1. simpl. destruct (LinDec_eq x h1).*)
+Restart. Check well_founded_induction.
+  intros A x l1 l2.
+  apply (@well_founded_induction (list A) _ (lengthOrder_wf A)
+    (fun l3 => l3 = l1 ++ l2 -> nb_occ A x (l1 ++ l2) = nb_occ A x (l2 ++ l1))).
+  intros; subst.
+Abort.
 
 Lemma perm_app : forall (A : LinDec) (l1 l2 : list A),
     perm A (l1 ++ l2) (l2 ++ l1).
@@ -100,21 +210,5 @@ Proof.
     simpl. intro. rewrite app_nil_r. apply perm_refl.
     simpl. induction l2 as [| h' t'].
       simpl. rewrite app_nil_r. apply perm_refl.
-      simpl. SearchAbout perm. Print perm.
-
-Lemma perm_lemma : forall (A : LinDec) (h : A) (t l1 l2 : list A),
-    perm A t (l1 ++ l2) -> perm A (h :: t) (l1 ++ h :: l2).
-Proof.
-  intros.
-
-Program Fixpoint qs' (A : LinDec) (l : list A) {measure (length l)}
-    : {l' : list A | perm A l l'} :=
-match l with
-    | nil => nil
-    | h :: t => qs' A (filter (fun x : A => leqb x h) t) ++ [h]
-             ++ qs' A (filter (fun x : A => negb (leqb x h)) t)
-end.
-Next Obligation. constructor. Qed.
-Next Obligation. simpl. unfold lt. auto. Qed.
-Next Obligation. simpl. unfold lt. auto. Qed.
-Next Obligation. *)
+      simpl.
+Abort.
