Mergesort.v
@@ -15,33 +15,6 @@ Fixpoint merge (A : LinDec) (l1 : list A) {struct l1} : list A -> list A :=
             else h2 :: f t2
     end.
 
-(*Theorem merge_eq1 : forall (A : LinDec) (h1 h2 : A) (t1 t2 : list A),
-  @leq A h1 h2 -> merge A (h1 :: t1) (h2 :: t2) = h1 :: merge A t1 (h2 :: t2).
-Proof.
-  intros. simpl. Check leq_total_dec. Print sumbool.*)
-
-
-Eval compute in merge natle [1; 2; 3] [4; 5; 6].
-
-Fixpoint merge' {A : LinDec} (n : nat) (l1 l2 : list A) : option (list A) :=
-match n, l1, l2 with
-    | 0, _, _ => None
-    | _, nil, _ => Some l2
-    | _, _, nil => Some l1
-    | S n', h :: t, h' :: t' =>
-        if leq_dec h h'
-        then match merge' n' t l2 with
-            | None => None
-            | Some m => Some (h :: m)
-        end
-        else match merge' n' l1 t' with
-            | None => None
-            | Some m => Some (h' :: m)
-        end
-end.
-
-Eval compute in merge' 10 [1; 2; 3] [4; 5; 6].
-
 Hint Constructors sorted.
 
 Theorem merge_sorted : forall (A : LinDec) (l1 l2 : list A),
@@ -61,82 +34,7 @@ Proof.
         destruct (leq_total_dec x x0); auto.
           destruct (leq_total_dec y x0); simpl; auto.
       simpl. destruct (leq_total_dec x x0).
-        
-
-assert (sorted A (y0 :: l0) -> sorted A (merge A (y :: l) (y0 :: l0))).
-        intro. clear H3.
 Abort.
-
-Theorem merge_sorted' : forall (A : LinDec) (n : nat) (l1 l2 l : list A),
-    sorted A l1 -> sorted A l2 -> merge' n l1 l2 = Some l ->
-    sorted A l.
-Proof.
-  induction 1; intros.
-    destruct n; inversion H0; subst; auto.
-    destruct n, l2; inversion H0; subst. constructor.
-      case_eq (leq_dec x c); intros eq' eq; rewrite eq in *.
-        destruct n; inversion H2; constructor; auto.
-        destruct n, l2; inversion H2. constructor. auto.
-  
-Abort. (*
-  induction n as [| n']; intros.
-    inversion H1.
-    induction H.
-      inversion H1; subst. assumption.
-      apply (IHn' [x] l2). constructor. auto. rewrite <- H1. destruct n'.
-        simpl in *. destruct l2. inversion H1.
-  induction 1. Print merge_func.
-Abort.*)
-
-Program Fixpoint merge2 (A : LinDec) (l1 l2 : list A)
-    {measure (length l1 + length l2)} : list A :=
-match l1, l2 with
-    | nil, _ => l2
-    | _, nil => l1
-    | h :: t, h' :: t' => if leq_dec h h'
-        then h :: (merge2 A t l2)
-        else h' :: (merge2 A l1 t')
-end.
-Next Obligation. simpl; omega. Defined.
-
-Eval compute in merge2 natle [1; 2; 3] [4; 5; 6].
-
-(*Theorem merge_eq : forall (A : LinDec) (l1 l2 : list A),
-    merge A l1 l2 = match l1, l2 with
-        | nil, _ => l2
-        | _, nil => l1
-        | h :: t, h' :: t' => if leq_dec h h'
-        then h :: (merge A t (h' :: t'))
-        else h' :: (merge A (h :: t) t')
-    end.
-Proof.
-  induction l1 as [| h t].
-    destruct l2; compute; trivial.
-    (*intro l2. generalize dependent t. generalize dependent h.*)
-    induction l2 as [| h' t']; intros.
-      compute. trivial.
-      destruct (leq_dec h h').
-        rewrite IHt. destruct t. compute. simpl. compute. simpl.*)
-
-(*Definition merge' : forall (A : LinDec) (l : list A * list A), list A.
-Proof. intro.
-  apply Fix with (fun l l' => length (fst l) + length (snd l) <
-    length (fst l') + length (snd l')).
-    red. intro. constructor. intros.
-      destruct a as [a1 a2], y as [y1 y2].
-      simpl in H. induction a1, a2, y1, y2; simpl in *;
-      try (inversion H; fail).
-        constructor. inversion 1.
-        constructor. simpl.
-      
-  Focus 2. exact (@nil A).
-  intros.
-  destruct l1 as [| h t].
-    exact l2.
-    destruct l2 as [| h' t'].
-      exact (h :: t).
-      destruct (leq_dec h h').
-        refine (X *)
 
 Fixpoint take {A : Type} (n : nat) (l : list A) : list A :=
 match n, l with
@@ -187,6 +85,7 @@ Qed.
 Require Import Arith.
 Require Import Div2.
 
+(* Mergesort using Program Fixpoint. *)
 Program Fixpoint msPF (A : LinDec) (l : list A) 
     {measure (length l)} : list A :=
 match l with
@@ -209,23 +108,14 @@ Next Obligation.
   split; repeat intro; inversion H3.
 Defined.
 
-Fixpoint aux (A : LinDec) (l : list (list A)) : list (list A) :=
-match l with
-    | [] => []
-    | [l'] => [l']
-    | l1 :: l2 :: t => merge A l1 l2 :: aux A t
-end.
-
-(*Eval compute in merge natle (qs natle [5; 2; 8]) (qs natle [6; 4; 9]).*)
-Eval compute in aux natle [[5; 2; 8]; [1; 4; 9]].
+Eval compute in msPF natle testl.
 
 (* Mergesort using Function. *)
-
 Function msFun (A : LinDec) (l : list A) {measure length l} : list A :=
 match l with
     | [] => []
     | [x] => [x]
-    | l' => 
+    | l' =>
       let n := div2 (length l') in
       let l1 := take n l' in
       let l2 := drop n l' in
@@ -238,6 +128,41 @@ Defined.
 
 Eval compute in msFun natle testl.
 
+(* Mergesort using fuel recursion. *)
+Fixpoint msFuel' (A : LinDec) (n : nat) (l : list A) : list A :=
+match n, l with
+    | 0, _ => []
+    | _, [] => []
+    | _, [x] => [x]
+    | S n', l' =>
+        let n := div2 (length l') in
+        let l1 := take n l' in
+        let l2 := drop n l' in
+        merge A (msFuel' A n' l1) (msFuel' A n' l2)
+end.
+
+Eval compute in msFuel' natle 5 testl.
+
+(* Mergesort using well-founded recursion and refine. *)
+Definition msWfRef (A : LinDec) : list A -> list A.
+refine (Fix (@lengthOrder_wf A) _
+(fun (l : list A) =>
+match l with
+    | [] => fun _ => []
+    | [x] => fun _ => [x]
+    | x :: y :: l' => fun msWf =>
+        let n := div2 (length (x :: y :: l')) in
+        let l1 := take n (x :: y :: l') in
+        let l2 := drop n (x :: y :: l') in merge A (msWf l1 _) (msWf l2 _)
+end)).
+Proof.
+  all: unfold l1, l2, n.
+    apply take_length2. apply lt_div2. simpl. omega.
+    apply drop_length2; simpl.
+      omega.
+      inversion 1.
+Defined.
+
 (* Mergesort using Bove-Capretta *)
 
 Inductive msDom {A : LinDec} : list A -> Type :=
@@ -247,13 +172,13 @@ Inductive msDom {A : LinDec} : list A -> Type :=
         msDom (take (div2 (length l)) l) ->
         msDom (drop (div2 (length l)) l) -> msDom l.
 
-Fixpoint ms_aux {A : LinDec} {l : list A} (dom : msDom l) : list A :=
+Fixpoint msBC' {A : LinDec} {l : list A} (dom : msDom l) : list A :=
 match dom with
     | msDom0 => []
     | msDom1 x => [x]
     | msDom2 l dom1 dom2 =>
-        let l1 := ms_aux dom1 in
-        let l2 := ms_aux dom2 in merge A l1 l2
+        let l1 := msBC' dom1 in
+        let l2 := msBC' dom2 in merge A l1 l2
 end.
 
 Theorem msDom_all : forall (A : LinDec) (l : list A), msDom l.
@@ -265,7 +190,7 @@ Proof.
       apply ms. apply drop_length2. simpl. omega. inversion 1.
 Defined.
 
-Definition ms {A : LinDec} (l : list A) : list A :=
-    ms_aux (msDom_all A l).
+Definition msBC (A : LinDec) (l : list A) : list A :=
+    msBC' (msDom_all A l).
 
-Eval compute in @ms natle testl.
+Eval compute in msBC natle testl.
